\documentclass[11pt]{article}
\begin{document}

\section*{Backward Propagation}
\subsection*{R$^{(3)}$}
$$r^{(3)}=\frac{\partial E(w)}{\partial a^{(3)}} = \frac{-t}{e^{ta^{(3)}}+1}$$

\subsection*{R$^{(2)}$}
$$ r^{(2)}_{q} = \frac{\partial E(w)}{\partial a^{(2)}_q} = \frac{\partial E(w)}{\partial a^{(3)}}\frac{\partial a^{(3)}}{\partial a^{(2)}_q}  $$
\subsubsection*{L}
$$r^{(2)}_{L} = r^{(3)} \frac{(w^{(3)})^T \cdot a_{LR}^{(2)} \cdot e^{a_R^{(2)}+a_L^{(2)}}}{(e^{a_R^{(2)}}+1)(e^{a_L^{(2)}}+1)^2}$$

\subsubsection*{R}
$$r^{(2)}_{R} =r^{(3)} \frac{(w^{(3)})^T \cdot a_{LR}^{(2)} \cdot e^{a_R^{(2)}+a_L^{(2)}}}{(e^{a_L^{(2)}}+1)(e^{a_R^{(2)}}+1)^2}$$

\subsubsection*{LR}
$$r^{(2)}_{LR} =r^{(3)} \frac{(w^{(3)})^T}{(e^{-a_L^{(2)}}+1)(e^{-a_R^{(2)}}+1)}$$

\subsection*{R$^{(1)}$}
$$ r^{(1)}_{q} = \frac{\partial E(w)}{\partial a^{(1)}_q} = \sum_{p\in\{L, R, LR\}} \frac{\partial E(w)}{\partial a_p^{(2)}}\frac{\partial a^{(2)}_p}{\partial a^{(1)}_q}  $$
\subsubsection*{L}
$$r^{(1)}_{L} = \sum_{i=1}^{H2} r^{(2)} ( (w_{L}^{(2)})^T\cdot sech(a_{L,i}^{(1)}) + (w_{LR,i}^{(2)})^T\cdot sech(a_{L}^{(1)}) ) $$

\subsubsection*{R}
$$r^{(1)}_{R} =  \sum_{i=1}^{H2}  r^{(2)} ( (w_{R}^{(2)})^T\cdot sech(a_{R,i}^{(1)}) + (w_{LR,i}^{(2)})^T\cdot sech(a_{R}^{(1)}) ) $$

\end{document}
